LeanBoogie/ITree/ITree0W.lean
@@ -14,33 +14,32 @@ abbrev ITree0 (A : Type) := ITree Empty A
 def Converges (a : A) (t : ITree0 A) : Prop := t ~~ .ret a
 def Diverges (t : ITree0 A) : Prop := t ~~ spin
 
-/-- The predicate `P` respects equivalence up to tau. -/
-def RespEutt (P : ITree0 A -> Prop) : Prop := ∀t1 t2 : ITree0 A, Eutt t1 t2 -> P t1 -> P t2
+-- /-- The predicate `P` respects equivalence up to tau. -/
+-- def RespEutt (P : ITree0 A -> Prop) : Prop := ∀t1 t2 : ITree0 A, Eutt t1 t2 -> P t1 -> P t2
 
 /-- Source: https://lag47.github.io/assets/pdf/dissertation.pdf definition 9,
   and the Interaction Trees repo `PureITreeDijkstra.v` definition `monotonici`.  -/
-def Monotonic (w : (p : ITree0 A -> Prop) -> (_ : RespEutt p) -> Prop) : Prop :=
-  (p1 p2 : ITree0 A -> Prop) -> {h1 : RespEutt p1} -> {h2 : RespEutt p2} ->
-      (∀t : ITree0 A, p1 t -> p2 t) ->
-        @w p1 h1 ->
-        @w p2 h2
+def Monotonic (w : (p : ITree0 A -> Prop) -> Prop) : Prop :=
+  (p1 p2 : ITree0 A -> Prop) ->
+    (∀t : ITree0 A, p1 t -> p2 t) ->
+      @w p1 -> @w p2
 
 /-- Specification monad for eventless interaction trees. In the Dijkstra Monads for ever paper,
   this is called `DelaySpec`. We require the specification to adhere to some properties (mono, respeutt)
   but that is not very relevant for generating verification conditions.
   You should be able to pretend this is just `def ITree0W (A) := (ITree0 A -> Prop) -> Prop`. -/
-def ITree0W (A : Type) := (w : (p : ITree0 A -> Prop) -> (_ : RespEutt p) -> Prop) ×' Monotonic w
+def ITree0W (A : Type) := (w : (ITree0 A -> Prop) -> Prop) ×' Monotonic w
 
 def ITree0W.pure {A   : Type} (a : A) : ITree0W A := ⟨
-  fun (post : ITree Empty A -> Prop) _ => post (Pure.pure a),
-  fun p1 p2 h1 _ t h => by simp_all only⟩
+  fun (post : ITree Empty A -> Prop) => post (Pure.pure a),
+  fun p1 p2 _ _ => by simp_all only⟩
 
 def ITree0W.bind {A B : Type} (wa : ITree0W A) (wb : A -> ITree0W B) : ITree0W B := ⟨
-  fun (post : ITree Empty B -> Prop) hpost =>
-    wa.1 (fun ta => (∃a:A, Converges a ta ∧ (wb a).1 post hpost) ∨ Diverges ta) (by sorry),
+  fun (post : ITree Empty B -> Prop) =>
+    wa.1 (fun ta => (∃a:A, Converges a ta ∧ (wb a).1 post ) ∨ Diverges ta),
   by
     unfold Converges Diverges
-    intro p1 p2 p1h p2h t h
+    intro p1 p2 t h
     unfold ITree0W at wa wb
     obtain ⟨wa, wah⟩ := wa
     -- obtain ⟨wb, wbh⟩ := wb ?a
@@ -56,10 +55,10 @@ instance : LawfulMonad ITree0W := sorry
 
 -- ## Morphism θ from ITree0 to ITree0W
 
-def ITree0.θ (t : ITree0 A) : ITree0W A := ⟨fun post _hpost => post t, by intro _ _ _ _ _ _; simp_all only⟩
+def ITree0.θ (t : ITree0 A) : ITree0W A := ⟨fun post => post t, by intro _ _ _ _; simp_all only⟩
 instance : Theta ITree0 ITree0W := ⟨ITree0.θ⟩
 
-def ITree0W.le (w1 w2 : ITree0W A) : Prop := ∀p, (hp : RespEutt p) -> w2.1 p hp -> w1.1 p hp
+def ITree0W.le (w1 w2 : ITree0W A) : Prop := ∀p, w2.1 p -> w1.1 p
 instance : LE (ITree0W A) := ⟨ITree0W.le⟩
 
 theorem ITree0.θ_pure : θ (return a) = return a := rfl
@@ -89,8 +88,8 @@ theorem θ_if {t e : ITree0 A} [Decidable c] : θ (if c then t else e) = if c th
 set_option linter.unusedVariables false in
 /-- Source: [DM4Ever] figure 4 `loop_invar_sound`, as well as in `DelaySpecMonad.v` definitino `loop_invar`. -/
 theorem loop_invar (body : A -> ITree0 (A ⊕ B)) (a₀ : A)
-  (P : ITree0 B -> Prop) {P_eutt : RespEutt P}
-  (Inv : ITree0 (A ⊕ B) -> Prop) {Inv_eutt : RespEutt P}
+  (P : ITree0 B -> Prop)
+  (Inv : ITree0 (A ⊕ B) -> Prop)
   (start : Inv (body a₀))
   (step : ∀r, Inv r -> Inv (r >>= iter_lift body))
   (stop : ∀t, Inv (t >>= fun b => return .inr b) -> P t)
