LeanBoogie/Mem.lean
@@ -30,7 +30,7 @@ def Mem.update (v : String) (f : Int -> Int) : ITree MemEv Unit
 -/
 
 /-- Transforms memory events into state monad actions. -/
-def interp (tm : ITree MemEv A) : Boogie Empty A := fun s₀ =>
+def interp (tm : ITree MemEv A) : Boogie A := fun s₀ =>
   ITree.corec (fun ⟨tm, s⟩ =>
     match tm.dest with
     | .ret a => .ret (a, s)
@@ -46,18 +46,18 @@ theorem interp_pure : interp (pure x) ~=~ pure x := sorry!
 theorem interp_ret : interp (.ret x) ~=~ pure x := interp_pure
 
 theorem interp_bind {ta : ITree MemEv A} {tb : A -> ITree MemEv B}
-  : interp (bind ta tb) ~=~ bind (interp ta) (fun a => interp (tb a))
+  : interp (ta >>= tb) = (interp ta) >>= (fun a => interp (tb a))
   := sorry!
 
 
 /-- Convenience mix of `interp_bind` and `bind_state_pull`. -/
 theorem interp_bind_pull {ta : ITree MemEv A} {tb : A -> ITree MemEv B}
-  : interp (ITree.bind ta tb) s ~~ ITree.bind (interp ta s) (fun x => interp (tb x.1) x.2)
+  : interp (ITree.bind ta tb) s = ITree.bind (interp ta s) (fun x => interp (tb x.1) x.2)
   := sorry!
 
 
 theorem interp_iter {body : A -> ITree MemEv (A ⊕ B)} {a₀ : A}
-  : interp (ITree.iter body a₀) ~=~ Boogie.iter (fun (a : A) => interp (body a)) a₀
+  : interp (ITree.iter body a₀) = Boogie.iter (fun (a : A) => interp (body a)) a₀
   := sorry!
 
 -- theorem interpk_iter {body : A -> ITree MemEv (A ⊕ B)} {a₀ : A}
@@ -65,12 +65,12 @@ theorem interp_iter {body : A -> ITree MemEv (A ⊕ B)} {a₀ : A}
 --   : interpk (ITree.iter body) ~~=~~ Boogie.iter (interpk body)
 --   := by sorry
 
-theorem interp_read : interp (Mem.read x) ~=~ Boogie.read x := sorry!
-theorem interp_write : interp (Mem.write x val) ~=~ (Boogie.write x val) := sorry!
+theorem interp_read : interp (Mem.read x) = Boogie.read x := sorry!
+theorem interp_write : interp (Mem.write x val) = (Boogie.write x val) := sorry!
 
-theorem interp_ite [Decidable φ] : interp (if φ then t else e) ~=~ (if φ then interp t else interp e) := sorry!
+theorem interp_ite [Decidable φ] : interp (if φ then t else e) = (if φ then interp t else interp e) := sorry!
 
-theorem interp_ite' : interp (ITree.ite c t e) ~=~ (do let c <- interp c; if c then interp t else interp e :) := sorry!
+theorem interp_ite' : interp (ITree.ite c t e) = (do let c <- interp c; if c then interp t else interp e :) := sorry!
 
 -- theorem interp_cat {f : KTree MemEv A B} {g : KTree MemEv B C}
 --   : interp (f a >>> g) ~~ (interp f >>> interpK g) a := sorry
