LeanBoogie/Woogie.lean
@@ -19,19 +19,19 @@ open ITree
   However, because `ITree0W` comes with some additional ballast such as monotonicity,
   it is a little uglier still:
   ```
-  (BoogieState →
-    (w : (p : ITree Empty (A × BoogieState) → Prop) -> RespEutt p → Prop) ×' Monotonic w)
+  BoogieState →
+    @PSigma ((ITree Empty (A × BoogieState) → Prop) -> Prop) (Monotonic w)
   ```
 -/
 def Woogie : Type -> Type := StateT BoogieState ITree0W
 
 example : Woogie A =
   (BoogieState →
-    (w : (p : ITree Empty (A × BoogieState) → Prop) -> RespEutt p → Prop) ×' Monotonic w)
+    (w : (ITree Empty (A × BoogieState) → Prop) -> Prop) ×' Monotonic w)
   := by rfl
 
 def Woogie.mk
-  (w : BoogieState -> (post : ITree0 (A × BoogieState) → Prop) -> RespEutt post → Prop)
+  (w : BoogieState -> (post : ITree0 (A × BoogieState) → Prop) -> Prop)
   (w_mono : (s : BoogieState) -> Monotonic (w s))
   : Woogie A
   := fun s => ⟨w s, w_mono s⟩
@@ -40,7 +40,7 @@ def Woogie.mk
 def Woogie.mk!
   (w : BoogieState -> (post : ITree0 (A × BoogieState) → Prop) → Prop)
   : Woogie A
-  := fun s => ⟨fun post _hpost => w s post, sorry⟩
+  := fun s => ⟨fun post => w s post, sorry⟩
 
 def Woogie.pure (a : A) : Woogie A := fun s => return (a, s)
 def Woogie.bind (a : Woogie A) (b : A -> Woogie B) : Woogie B := fun s => a s >>= fun a => b a.fst a.snd
@@ -52,31 +52,31 @@ instance : LawfulMonad Woogie := sorry
 
 def Woogie.read (v : String) : Woogie Int :=
   fun (s:BoogieState) => ⟨
-    fun (post) _ => post (.ret (s v, s)),
+    fun (post) => post (.ret (s v, s)),
     by unfold Monotonic; aesop
   ⟩
 
 def Woogie.write (v : String) (a : Int) : Woogie Unit :=
   fun s => ⟨
-    fun post _ => post (.ret ((), s.update v a)),
+    fun post => post (.ret ((), s.update v a)),
     by rw [Monotonic]; aesop
   ⟩
 
 /-- This is `θ_state` in DM4Ever. -/
-def Boogie.θ (b : Boogie Empty A) : Woogie A :=
+def Boogie.θ (b : Boogie A) : Woogie A :=
   fun s => ⟨
-    fun post _ => post (b s),
+    fun post => post (b s),
     by rw [Monotonic]; aesop
   ⟩
 
-instance : Theta (Boogie Empty) Woogie := ⟨Boogie.θ⟩
+instance : Theta Boogie Woogie := ⟨Boogie.θ⟩
 
 /-- Specification ordering [DM4Aall 3.1]. -/
-def Woogie.le (w1 w2 : Woogie A) : Prop := ∀s p, (hp : RespEutt p) -> (w2 s).1 p hp -> (w1 s).1 p hp
+def Woogie.le (w1 w2 : Woogie A) : Prop := ∀s p, (w2 s).1 p -> (w1 s).1 p
 instance : LE (Woogie A) := ⟨Woogie.le⟩
 
 theorem Boogie.θ_pure : θ (return a) = (return a) := rfl
-theorem Boogie.θ_bind {a : Boogie Empty A} {b : A -> Boogie Empty B}
+theorem Boogie.θ_bind {a : Boogie A} {b : A -> Boogie B}
   : θ (a >>= b) = (θ a >>= fun a => θ (b a))
   := by
     unfold θ
@@ -84,7 +84,7 @@ theorem Boogie.θ_bind {a : Boogie Empty A} {b : A -> Boogie Empty B}
     unfold Woogie.bind
     funext s
     congr
-    funext post hpost
+    funext post
     ext
     simp_all only [Prod.exists]
     constructor
@@ -98,12 +98,12 @@ theorem Boogie.θ_bind {a : Boogie Empty A} {b : A -> Boogie Empty B}
       | inr h_2 =>
         sorry
 
-instance : LawfulTheta (Boogie Empty) (Woogie) := ⟨Boogie.θ_pure, Boogie.θ_bind⟩
+instance : LawfulTheta Boogie Woogie := ⟨Boogie.θ_pure, Boogie.θ_bind⟩
 
-theorem Boogie.θ_read : θ (Boogie.read v) = (Woogie.read v) := by sorry
-theorem Boogie.θ_write : θ (Boogie.write v x) = (Woogie.write v x) := by sorry
+theorem Woogie.θ_read : θ (Boogie.read v) = (Woogie.read v) := by sorry
+theorem Woogie.θ_write : θ (Boogie.write v x) = (Woogie.write v x) := by sorry
 
-theorem Boogie.θ_ite [Decidable φ]
+theorem Woogie.θ_ite [Decidable φ] {t e : Boogie A}
   : θ (if φ then t else e)
   = (if φ then θ t else θ e)
   := by
@@ -111,29 +111,29 @@ theorem Boogie.θ_ite [Decidable φ]
   next h => simp_all only
   next h => simp_all only
 
-theorem Boogie.θ_ite' [Decidable φ]
+theorem Woogie.θ_ite' [Decidable φ] {t e : Boogie A}
   : θ (if φ then t else e)
-  = Woogie.mk! (fun s post => (φ -> (θ t s).1 post sorry) ∧ (¬φ -> (θ e s).1 post sorry))
+  = Woogie.mk! (fun s post => (φ -> (θ t s).1 post) ∧ (¬φ -> (θ e s).1 post))
   := by
   split
   next h => simp_all only [true_implies, not_true_eq_false, false_implies, and_true]; rfl
   next h => simp_all only [false_implies, not_false_eq_true, true_implies, true_and]; rfl
 
-def BoogV {A : Type} (w : Woogie A) (b : Boogie Empty A) : Prop := θ b <= w
+def BoogieV {A : Type} (w : Woogie A) (b : Boogie A) : Prop := θ b <= w
 
-theorem BoogV.ite [Decidable φ] {w : Woogie A}
-  (tru :  φ -> BoogV w t)
-  (fal : ¬φ -> BoogV w e)
-  : BoogV w (if φ then t else e)
+theorem BoogieV.ite [Decidable φ] {w : Woogie A}
+  (tru :  φ -> BoogieV w t)
+  (fal : ¬φ -> BoogieV w e)
+  : BoogieV w (if φ then t else e)
   := by aesop
 
-theorem BoogV.ite' [Decidable φ] {w : Woogie A} {t e : Boogie Empty A}
+theorem BoogieV.ite' [Decidable φ] {w : Woogie A} {t e : Boogie A}
   (tru :  φ -> θ t <= w)
   (fal : ¬φ -> θ e <= w)
   : θ (if φ then t else e) <= w
   := by aesop
 
-theorem BoogV.ite'' [Decidable φ] {w : Woogie A}
+theorem BoogieV.ite'' [Decidable φ] {w : Woogie A}
   (tru :  φ -> t <= w)
   (fal : ¬φ -> e <= w)
   : (if φ then t else e) <= w
